make more things contractive

theories/logrel_heaplang_sessions/rules/mutex.v
@@ -11,12 +11,12 @@ Section types.
   Definition lty_mutex (A : lty Σ) : lty Σ := Lty (λ w,
     ∃ (N : namespace) (γ : gname) (l : loc) (lk : val),
       ⌜ w = PairV lk #l ⌝
-      ∗ is_lock N γ lk (∃ inner, l ↦ inner ∗ A inner))%I.
+      ∗ is_lock N γ lk (∃ inner, l ↦ inner ∗ ▷ A inner))%I.
 
   Definition lty_mutexguard (A : lty Σ) : lty Σ := Lty (λ w,
     ∃ (N : namespace) (γ : gname) (l : loc) (lk : val) (v : val),
       ⌜ w = PairV lk #l ⌝
-      ∗ is_lock N γ lk (∃ inner, l ↦ inner ∗ A inner)
+      ∗ is_lock N γ lk (∃ inner, l ↦ inner ∗ ▷ A inner)
       ∗ locked γ ∗ l ↦ v)%I.
 End types.
 
@@ -25,6 +25,11 @@ Notation "'mutexguard' A" := (lty_mutexguard A) (at level 10) : lty_scope.
 
 Section properties.
   Context `{heapG Σ, lockG Σ}.
+
+  Global Instance lty_mutex_contractive : Contractive (@lty_mutex Σ _ _).
+  Proof. solve_contractive. Qed.
+  Global Instance lty_mutex_ne : NonExpansive (@lty_mutex Σ _ _).
+  Proof. solve_proper. Qed.
 
   Definition mutexalloc : val := λ: "x", (newlock #(), ref "x").
   Lemma ltyped_mutexalloc A:
@@ -37,7 +42,7 @@ Section properties.
     wp_alloc l as "Hl".
     wp_bind (newlock _).
     set (N := nroot .@ "makelock").
-    iAssert (∃ inner, l ↦ inner ∗ A inner)%I with "[Hl Hv]" as "Hlock".
+    iAssert (∃ inner, l ↦ inner ∗ ▷ A inner)%I with "[Hl Hv]" as "Hlock".
     { iExists v. iFrame "Hl Hv". }
     wp_apply (newlock_spec N with "Hlock").
     iIntros (lk γ) "Hlock".
@@ -52,8 +57,8 @@ Section properties.
     iIntros (vs) "HΓ /=".
     wp_apply wp_value.
     iIntros (m) "Hm".
-    iDestruct "Hm" as (N γ l lk ->) "#Hlock".
     rewrite /mutexacquire. wp_pures.
+    iDestruct "Hm" as (N γ l lk ->) "#Hlock".
     wp_bind (acquire _).
     wp_apply (acquire_spec N with "Hlock").
     iIntros "[Hlocked Hinner]".
@@ -75,13 +80,16 @@ Section properties.
     iIntros (w1) "Hw1".
     rewrite /mutexrelease. wp_pures.
     iIntros (w2) "Hw2".
+    wp_pures.
     iDestruct "Hw2" as (N γ l lk inner ->) "[#Hlock [Hlocked Hinner]]".
-    wp_pures. wp_store.
-    iAssert (∃ inner : val, l ↦ inner ∗ A inner)%I with "[Hinner Hw1]" as "Hinner".
+    wp_store.
+    iAssert (∃ inner : val, l ↦ inner ∗ ▷ A inner)%I with "[Hinner Hw1]" as "Hinner".
     { iExists w1. iFrame "Hinner Hw1". }
     wp_bind (release _).
-    wp_apply (release_spec N γ _ (∃ inner, l ↦ inner ∗ A inner)%I with "[Hlocked Hinner]").
-    { iFrame "Hlock Hlocked Hinner". }
+    wp_apply (release_spec N γ _ (∃ inner, l ↦ inner ∗ ▷ A inner)%I with "[Hlocked Hinner]").
+    { iFrame "Hlock Hlocked".
+      iDestruct "Hinner" as (v) "[Hl HA]".
+      iExists v. iFrame "Hl". iModIntro. iFrame "HA". }
     iIntros "_".
     wp_pures.
     iExists N, γ, l, lk. iSplit=> //.
